src/Goose/base.v
@@ -6,7 +6,9 @@ From RecoveryRefinement.Goose Require Export Machine.
 From RecoveryRefinement.Goose Require Export GoZeroValues.
 From RecoveryRefinement.Goose Require Export GoLayer.
 
-Import EqualDecNotation.
-Import ProcNotations. Open Scope proc.
+Export EqualDecNotation.
+Export ProcNotations. Open Scope proc.
+
+Open Scope string.
 
 Notation proc := (Proc.proc Op).
